sparse vector scaling

src/examples/Kuiper.Example.Sparse.fst
@@ -70,6 +70,138 @@ let sarray_live #et {| scalar et |} #len (s : sarray et len) : slprop =
   // (exists* v. s.elems |-> v) **
   // (exists* v. s.pos |-> v)
 
+
+inline_for_extraction noextract
+fn sarray_id
+  (#et : Type0) {| scalar et |}
+  (len : erased nat)
+  (a : sarray et len)
+  preserves gpu
+  preserves (exists* s. sarray_pts_to a s)
+{
+  with s.
+    assert(sarray_pts_to a s);
+  let mut i = 0sz;
+  while(FStar.SizeT.(!i <^ a.nnz))
+    invariant
+      (sarray_pts_to a s) **
+      (exists* i_v. i |-> i_v)
+  {
+    unfold (sarray_pts_to a s);
+    with v_elems. assert a.elems |-> v_elems;
+
+    let v = gpu_array_read a.elems !i;
+    gpu_array_write a.elems !i v;
+
+    with i_v.
+      assert i |-> i_v;
+      assert pure (Seq.equal v_elems (Seq.upd v_elems i_v v));
+
+    i := !i `SZ.add` 1sz;
+    
+    fold(sarray_pts_to a s);
+  }
+}
+
+let _id_u32 = sarray_id #u32 #_
+
+assume
+val zero_is_id
+  (#et:_) {| d : scalar et |}
+  (k : et)
+  : Lemma
+    (requires true)
+    (ensures k `d.mul` zero == zero /\ zero `d.mul` k == zero)
+
+let scale_seq
+  (#et:_) {| d : scalar et |}
+  (k : et)
+  (#len : nat)
+  (s : lseq et len)
+  : Pure (lseq et len)
+    (requires true)
+    (ensures fun s' -> forall i. Seq.index s' i == k `d.mul` Seq.index s i)
+=
+  let open FStar.Seq in
+
+  map_seq_len (mul k) s;
+  let s' = map_seq (mul k) s in
+  introduce forall i. index s' i == k `mul` index s i
+  with map_seq_index (mul k) s i;
+  s'
+
+let scale_unsparse
+  (#et:_) {| scalar et |}
+  (k : et)
+  (#nnz #len : nat)
+  (elems : lseq et nnz)
+  (pos   : lseq sz nnz{valid_pos len pos})
+  : Lemma
+    (requires true)
+    (ensures scale_seq k (unsparse nnz len elems pos) == unsparse nnz len (scale_seq k elems) pos)
+=
+  let open FStar.Seq in
+
+  let (nat_pos : seq nat) = map_seq SZ.v pos in
+  map_seq_len SZ.v pos;
+
+  let s = scale_seq k (unsparse nnz len elems pos) in
+  let s' = unsparse nnz len (scale_seq k elems) pos in
+  
+  introduce forall (i : nat{i < len}). Seq.index s i == Seq.index s' i
+  with
+    if Seq.mem i nat_pos
+      then ()
+      else zero_is_id k;
+
+  assert (s `equal` s')
+
+inline_for_extraction noextract
+fn sarray_scale
+  (#et : eqtype) {| scalar et |}
+  (k : et)
+  (len : erased nat)
+  (a : sarray et len)
+  (s : erased (lseq et len))
+  preserves gpu
+  requires sarray_pts_to a s
+  ensures sarray_pts_to a (scale_seq k s)
+{
+  unfold sarray_pts_to a s;
+
+  let mut i = 0sz;
+
+  with v_elems. assert a.elems |-> v_elems;
+  with v_pos. assert a.pos |-> v_pos;
+  
+  while(FStar.SizeT.(!i <^ a.nnz))
+    invariant
+      (exists* i_v v_elems'. 
+        i |-> i_v **
+        a.elems |-> v_elems' **
+        pure FStar.Seq.(
+          FStar.SizeT.(i_v <=^ a.nnz) /\ 
+          length v_elems' == a.nnz /\
+          forall (i : nat{i < a.nnz}).
+            (i < (SZ.v i_v) ==> index v_elems' i == k `mul` index v_elems i) /\
+            (i >= (SZ.v i_v) ==> index v_elems' i == index v_elems i)))
+  {
+    let v = gpu_array_read a.elems !i;
+    gpu_array_write a.elems !i (k `mul` v);
+    i := !i `SZ.add` 1sz;
+  };
+
+  with v_elems'. assert a.elems |-> v_elems';
+
+  assert pure FStar.Seq.(v_elems' `equal` scale_seq k v_elems);
+
+  scale_unsparse k #a.nnz #len v_elems v_pos;
+
+  fold sarray_pts_to a (scale_seq k s);
+}
+
+let _scale_u32 = sarray_scale #u32 #_
+
 inline_for_extraction noextract
 fn _add1
   (#et : Type0) {| scalar et |}
@@ -119,8 +251,7 @@ fn add1
     gpu_array_write a.elems !i v';
     i := !i `SZ.add` 1sz;
     with s'.
-      fold sarray_pts_to a s';
-    ()
+      fold sarray_pts_to a s'
   };
 }
 
